WeirdLogic/WLogic.lean
@@ -474,16 +474,175 @@ lemma weird_grmdisj_lemma_aux' (s' s : Set (α × β)) (H₃ HH H₁ H₂ : hhPr
   unfold LGTM.wp at h1 h2
   sorry
 
+-- lemma weird_hhwand (h1 h2 : hheap α) (H1 H2 : hhProp α) :
+--   H2 h2 →
+--   H1 h1 →
+--   hdisjoint h1 h2 →
+--   (H1 ∗ H2) (h1 ∪ h2) :=
+-- by
+--   move=> [? ![hW1 ?? [/hhimpl h1W hW2emp] /hW2emp /hunion_empty hU *] ]
+--   apply h1W ; exists h1, hW1
+--   sby srw hU
 
-lemma weird_grmdisj_lemma' (s' s : Set (α × β)) (sht_prog sht_lang : LGTM.SHT) :
-  sht_prog.s = ⟪0, s''⟫ ->
-  sht_lang.s = ⟪ 1, s⟫ ->
-  s' ⊆ s -> Disjoint sht_prog.s sht_lang.s ->
-  -- H₃ = HH  (H₁ ∗ H₂) ->
-  HH ∗ H₁ ==> LGTM.wp [sht_prog, ⟨⟪ 1, s \ s'⟫, sht_lang.ht ⟩ ] (fun _ h => ∀ ll ∈ s \ s', ∃ pp, pp ∈ s'' ∧ h ⟨1, ll ⟩= h ⟨0, pp⟩) ->
-  HH ∗ H₂ ==> LGTM.wp [sht_prog, ⟨⟪ 1, s'⟫, sht_lang.ht ⟩ ] (fun _ h => ∀ ll ∈ s', ∃ pp,  pp ∈ s'' ∧ h ⟨1, ll ⟩= h ⟨0, pp⟩) ->
-  HH ∗ H₁ ∗ H₂ ==> LGTM.wp [sht_prog, sht_lang]  (fun v h => ∀ ll ∈ s, ∃ pp, pp ∈ s'' ∧ h ⟨1, ll ⟩= h ⟨0, pp⟩) := by
+lemma union_heap_eq_l (h h1 h2 : hheap α ) :
+  h = h1 ∪ h2 ->
+  h1 a = h1 b ->
+  h a = h b := by
+  move=> hun pre
+  unfold Union.union instUnionHheap at hun
+  simp only [hun]
+  unfold hunion
+  apply Finmap.ext_lookup=> l /==
+  stop
+  rcases hh : Finmap.lookup l (h1 a ∪ h2 a) with ⟨⟩ | v₁
+  { srw Finmap.lookup_eq_none at hh
+    apply Finmap.lookup_union_right at h
+    srw h Option.merge_none_l=> // }
+  { have hh : l ∈ h₁ := by rw [← Finmap.lookup_isSome, h]=> //
+    apply dj at hh; srw Finmap.lookup_union_left_of_not_in=> //
+    srw -Finmap.lookup_eq_none at hh; rw [hh, h]=> // }
   sorry
+
+#check Finmap.lookup_union_left_of_not_in
+
+lemma union_heap_eq_r (h h1 h2 : hheap α ) :
+  h = h1 ∪ h2 ->
+  (∀ (a : α), Finmap.Disjoint (h1 a) (h2 a)) ->
+  h2 x = h2 y ->
+  h x = h y := by
+  move=> un dj pre
+  have djx:= dj x
+  have djy := dj y
+  rw [un]
+  stop
+  apply Finmap.ext_lookup=> l /==
+  simp
+  rcases hh : Finmap.lookup l (h1 x ∪ h2 x) with ⟨⟩ | v₁
+  stop
+  · srw Finmap.lookup_eq_none at hh
+    apply Eq.symm
+    apply Finmap.lookup_eq_none.mpr
+    simp
+  . apply Finmap.lookup_union_right at h
+    srw h Option.merge_none_l=> //
+    move=> pre2
+    cases pre2 with
+    | inl h11 => sorry
+    | inr h12 =>
+      rcases h12 with ⟨h_notin, h2_lookup⟩
+      right
+      constructor=>//
+
+
+set_option maxHeartbeats 1600000 in
+lemma weird_grmdisj_lemma' (s' s : Set (α × β)) (sht_prog sht_lang : LGTM.SHT) :
+  sht_prog.s = ⟪0, s'⟫ ->
+  sht_lang.s = ⟪ 1, s⟫ ->
+  Disjoint sht_prog.s sht_lang.s ->
+  s1 ∩ s2 = ∅ -> s1 ∪ s2 = s ->
+  s'1 ∩ s'2 = ∅ -> s'1 ∪ s'2 = s' ->
+  H₁ ==> LGTM.wp [⟨⟪ 0, s'1⟫, sht_prog.ht ⟩, ⟨⟪ 1, s1⟫, sht_lang.ht ⟩ ] (fun _ h => ∀ ll ∈ s1, ∃ pp, pp ∈ s'1 ∧ h ⟨1, ll ⟩= h ⟨0, pp⟩) ->
+  H₂ ==> LGTM.wp [⟨⟪ 0, s'2⟫, sht_prog.ht ⟩, ⟨⟪ 1, s2⟫, sht_lang.ht ⟩ ] (fun _ h => ∀ ll ∈ s2, ∃ pp,  pp ∈ s'2 ∧ h ⟨1, ll ⟩= h ⟨0, pp⟩) ->
+  H₁ ∗ H₂ ==> LGTM.wp [sht_prog, sht_lang]  (fun _ h => ∀ ll ∈ s, ∃ pp, pp ∈ s' ∧ h ⟨1, ll ⟩= h ⟨0, pp⟩) := by
+  move=> prog lang subs sp1 sp2 sp3 sp4 up1 up2
+  have subsht : LGTM.wp [sht_prog, sht_lang] (fun _ h => ∀ ll ∈ s, ∃ pp, pp ∈ s' ∧ h ⟨1, ll ⟩= h ⟨0, pp⟩) = LGTM.wp ([⟨⟪ 0, s'1⟫, sht_prog.ht ⟩, ⟨⟪ 1, s1⟫, sht_lang.ht ⟩ ] ++ [⟨⟪ 0, s'2⟫, sht_prog.ht ⟩, ⟨⟪ 1, s2⟫, sht_lang.ht ⟩]) (fun v h => ∀ ll ∈ s, ∃ pp, pp ∈ s' ∧ h ⟨1, ll ⟩= h ⟨0, pp⟩):= by
+    unfold LGTM.wp
+    simp
+    rw [prog,lang]
+    have sames : (⟪0, s'⟫ ∪ ⟪1, s⟫) = (⟪0, s'1⟫ ∪ (⟪1, s1⟫ ∪ (⟪0, s'2⟫ ∪ ⟪1, s2⟫))) := by
+      unfold labSet
+      simp
+      aesop
+    rw [← sames]
+    apply hwp_ht_eq
+    unfold Set.EqOn
+    intro x
+    move=> h
+    simp;
+    scase_if=>//==
+    · move=> h1 h2
+      scase_if=>/==
+      move=> h3
+      scase_if=>//
+    · move=> h1
+      scase_if=>// h2
+      · simp
+        rcases h2 with ⟨h21,h22⟩
+        scase_if
+        aesop
+      · apply not_and.mp at h2
+        scase_if
+        · simp
+          move=> h3
+          specialize h1 h3
+          aesop
+        · simp
+          move=> h3
+          scase_if
+          · aesop
+          · simp; move => h4
+            scase_if
+            · simp; move=> h5; aesop
+            · simp; move=> h6;
+              scase_if
+              simp; move=> h7; specialize h2 h7;
+              aesop
+  rw [subsht]
+  let Qmid : hhProp (α × β)ˡ:= (fun h => ∀ ll ∈ s1, ∃ pp, pp ∈ s'1 ∧ h ⟨1, ll ⟩= h ⟨0, pp⟩)
+  set Qp1 : hval (α × β)ˡ → hhProp (α × β)ˡ:= fun _ => fun h ↦ ∀ ll ∈ s2, ∃ pp ∈ s'2, h ⟨1, ll⟩ = h ⟨0, pp⟩
+  set B : hhProp (α × β)ˡ:= fun  h => ∀ ll ∈ s1, ∃ pp, pp ∈ s'1 ∧ h ⟨1, ll ⟩= h ⟨0, pp⟩
+  set B' : hval (α × β)ˡ → hhProp (α × β)ˡ:= fun _ => B
+  intro hv
+  move=> pre
+  apply weird_wp_conseq (Q1 := whqstar Qp1 B)
+  {
+    unfold whqstar B Qp1
+    unfold hqimpl hhimpl hhstar
+    intro hv0 hh
+    -- dsimp
+    simp
+    move=> hv1 pp1 hv2 pp2 hhv a1 aa1 bb1 hab
+    specialize pp1 aa1 bb1
+    specialize pp2 aa1 bb1
+    by_cases h_in_s2 : (aa1, bb1) ∈ s2
+    · rcases pp1 h_in_s2 with ⟨a, b, ⟨hab', heq_hv1⟩⟩
+      use a; use b
+      constructor
+      · aesop
+      · apply union_heap_eq_l (h := hh) (h1 := hv1) (h2 := hv2)=>//
+    · have h_in_s1 : (aa1, bb1) ∈ s1 := by
+        rw [←sp2, Set.mem_union] at hab
+        exact hab.resolve_right h_in_s2
+      rcases pp2 h_in_s1 with ⟨a, b, ⟨hab', heq_hv2⟩⟩
+      use a, b
+      constructor
+      · aesop
+      · apply union_heap_eq_r (h := hh) (h1 := hv1) (h2 := hv2)=>//
+  }
+  apply well_formed_sequ_lemma (R := H₁ ∗ H₂) (H := fun x => B ∗ H₂)
+  { simp; apply disjoint_label_set.mpr; simp }
+  { simp; apply disjoint_label_set.mpr; simp }
+  { simp
+    constructor
+    · constructor
+      · apply disjoint_label_set.mpr; simp; apply Set.disjoint_iff_inter_eq_empty.mpr; exact sp3
+      · apply disjoint_label_set.mpr; simp
+    · constructor
+      · apply disjoint_label_set.mpr; simp
+      · apply disjoint_label_set.mpr; simp; apply Set.disjoint_iff_inter_eq_empty.mpr; exact sp1
+  }
+  { apply hhimpl_frame_l (hH₃ := H₂) at up1
+    apply hhimpl_trans=>//
+    apply LGTM.wp_frame}
+  { intro hv
+    apply hhimpl_frame_r (hH₃ := B) at up2
+    apply hhimpl_trans=>//
+    srw hhstar_comm
+    apply LGTM.wp_frame
+  }
+  { exact pre}
+
+
 
 #check hhand
 
